Utils.v
@@ -1,0 +1,9 @@
+From Coq Require Import List.
+Import ListNotations.
+
+Fixpoint nth_opt {A: Type} (n: nat) (l: list A): option A :=
+  match n, l with
+  | _, nil => None
+  | 0, x::_ => Some x
+  | S n', _::q => nth_opt n' q
+  end.
