warblreequiv/LWEquivMain.v
@@ -1,80 +1,54 @@
 From Warblre Require Import Semantics Frontend Result.
-From Linden Require Import LindenParameters RegexpTranslation Regex Chars Tree Groups Semantics.
+From Linden Require Import LindenParameters RegexpTranslation Regex Chars Tree Groups Semantics Utils.
 From Coq Require Import List.
 Import ListNotations.
 
 Definition equiv_flags: RegExpFlags := {|
-    RegExpFlags.d := true;
-    RegExpFlags.g := false;
-    RegExpFlags.i := false;
-    RegExpFlags.m := false;
-    RegExpFlags.s := false;
-    RegExpFlags.u := tt;
-    RegExpFlags.y := true
-    |}.
+  RegExpFlags.d := true;
+  RegExpFlags.g := false;
+  RegExpFlags.i := false;
+  RegExpFlags.m := false;
+  RegExpFlags.s := false;
+  RegExpFlags.u := tt;
+  RegExpFlags.y := true
+  |}.
 
 Definition warblre_exec (r: regex) (s: string): option ExecResult :=
-    let warblre_r := to_warblre_regex r in
-    match regExpInitialize (specParameters := LindenParameters) warblre_r equiv_flags with
+  let warblre_r := to_warblre_regex r in
+  match regExpInitialize (specParameters := LindenParameters) warblre_r equiv_flags with
+  | Error _ => None
+  | Success rei =>
+    match regExpBuiltinExec rei s with
     | Error _ => None
-    | Success rei =>
-        match regExpBuiltinExec rei s with
-        | Error _ => None
-        | Success res => Some res
-        end
-    end.
-
-Fixpoint nth_opt {A: Type} (n: nat) (l: list A): option A :=
-    match n, l with
-    | _, nil => None
-    | 0, x::_ => Some x
-    | S n', _::q => nth_opt n' q
-    end.
+    | Success res => Some res
+    end
+  end.
 
 Definition group_maps_equal (li: list (option (nat*nat))) (l: option leaf) : Prop :=
-    match l with
-    | None => False
-    | Some lf => forall n: nat, match nth_opt n li with
-        | None | Some None => get_begin lf n = None /\ get_end lf n = None
-        | Some (Some (bg, ed)) => get_begin lf n = Some bg /\ get_end lf n = Some ed
-        end
-    end.
-
-Fixpoint num_groups (r: regex): nat :=
-    match r with
-    | Epsilon | Character _ => 0
-    | Disjunction r1 r2 => num_groups r1 + num_groups r2
-    | Sequence r1 r2 => num_groups r1 + num_groups r2
-    | Star _ r1 => num_groups r1
-    | Group _ r1 => S (num_groups r1)
-    end.
-
-Inductive well_parenthesized' : nat -> regex -> Prop :=
-| wp_eps: forall n, well_parenthesized' n Epsilon
-| wp_char: forall n cd, well_parenthesized' n (Character cd)
-| wp_disj: forall n r1 r2, well_parenthesized' n r1 -> well_parenthesized' (num_groups r1 + n) r2 -> well_parenthesized' n (Disjunction r1 r2)
-| wp_seq: forall n r1 r2, well_parenthesized' n r1 -> well_parenthesized' (num_groups r1 + n) r2 -> well_parenthesized' n (Sequence r1 r2)
-| wp_star: forall n greedy r, well_parenthesized' n r -> well_parenthesized' n (Star greedy r)
-| wp_group: forall n r, well_parenthesized' (S n) r -> well_parenthesized' n (Group (S n) r).
-
-Definition well_parenthesized (r: regex) := well_parenthesized' 0 r.
+  match l with
+  | None => False
+  | Some lf => forall n: nat, match nth_opt n li with
+    | None | Some None => get_begin lf n = None /\ get_end lf n = None
+    | Some (Some (bg, ed)) => get_begin lf n = Some bg /\ get_end lf n = Some ed
+    end
+  end.
 
 Theorem linden_warblre_equiv:
-    forall r s t,
-    well_parenthesized r ->
-    backtree (Group 0 r) s t ->
-    match warblre_exec r s with
-    | None => False
-    | Some res => match res with
-        | Null _ => first_branch t = None
-        | Exotic {| ExecArrayExotic.indices_array := ia |} _ =>
-            match ia with
-            | None => False
-            | Some li => group_maps_equal li (first_branch t)
-            end
-        end
-    end.
+  forall r s t,
+  well_parenthesized r ->
+  backtree (Group 0 r) s t ->
+  match warblre_exec r s with
+  | None => False
+  | Some res => match res with
+    | Null _ => first_branch t = None
+    | Exotic {| ExecArrayExotic.indices_array := ia |} _ =>
+      match ia with
+      | None => False
+      | Some li => group_maps_equal li (first_branch t)
+      end
+    end
+  end.
 Proof.
-    intros r s t Hwellparen Hbt.
-    unfold warblre_exec.
+  intros r s t Hwellparen Hbt.
+  unfold warblre_exec.
 Abort.
